You see something peculiar? Then you got it right: we can solve it similar to a linear function, replacing $t$ by a constant and this is what Cauchy's problem tries to prove: 
$$\left\{\begin{array}{l}\ y'=a(t)y+b(t)\\ \ y(t_0)=c\end{array}\right.$$

###### Example:
![[Pasted image 20230107160847.png]]

Here, we're considering that $a(t) = 0$ and based of Cauchy's problem: $y_0$ is a constant.  From this, we can easily assume $y' = t^2$, which's primitive corresponds to ${t^3\over 3} + 1$, that fully fits $y$ definition, as $y(t) = 1; t = 0$ verifies.