Gauss's lemma (the one where seeing now) is strongly tied to Bachet-Bezout's theorem. It states that: 
$$\left.\begin{array}{r}
a | bc \\
a \land b = 1
\end{array}\right\} \implies a |c$$

It is a consequence based of the theorem, as if we multiply $a \land b$ by $c$ we end up with $c$ (as the lemma implies that $a \land b = 1$). 

Therefore we have the following expression: $au \cdot c + bv \cdot c = \not 1\cdot c$.

Therefore $a$ logically divides $auc$ and based on the lemma $a$ supposedly divides $bc$ and therefore $bcv$. So $a$ divides the $a(uc) + (bc) v$ statement left- and right- hand sides, which logically leads to $a | a(uc) + (bc) v = c$.

![[Pasted image 20221225172106.png]]